Fixed Game Hop 2 -> 3 with some intermediate games and use of DMapSampling. Should still clean up though.

Security/SaberRqSecurity.ec
@@ -114,7 +114,7 @@ module Game0(A : Adversary) = {
       (m0, m1) <@ A.choose(pk_encode (sd, b));
 
       s' <$ dsmallRq_vec;
-      b' <- scaleRqv2Rpv (( trmx _A) *^ s' + h);
+      b' <- scaleRqv2Rpv ((trmx _A) *^ s' + h);
       v' <- (dotp b (Rqv2Rpv s')) + (Rq2Rp h1);
       cmu <- scaleRp2R2t (v' + (shl_enc (m_decode (if u then m1 else m0)) (ep - 1)));
       
@@ -147,7 +147,7 @@ module Game1(A : Adversary) = {
       (m0, m1) <@ A.choose(pk_encode (sd, b));
 
       s' <$ dsmallRq_vec;
-      b' <- scaleRqv2Rpv (( trmx _A) *^ s' + h);
+      b' <- scaleRqv2Rpv ((trmx _A) *^ s' + h);
       v' <- (dotp b (Rqv2Rpv s')) + (Rq2Rp h1);
       cmu <- scaleRp2R2t (v' + (shl_enc (m_decode (if u then m1 else m0)) (ep - 1)));
       
@@ -425,13 +425,13 @@ lemma Equivalence_SaberINDCPA_Game0 &m (A <: Adversary) :
       =
       `| Pr[Game0(A).main() @ &m : res] - 1%r /2%r |.
 proof.
-  have -> //: Pr[CPA(Saber_PKE_Scheme, A).main() @ &m : res] = Pr[Game0(A).main() @ &m : res].
-  + byequiv => //.
-    proc; inline *. 
-    swap {1} 7 -6.
-    call (_ : true); auto; call (_: true); auto.
-    progress; first do! congr; by rewrite pk_enc_dec_inv.
-    - by rewrite (eq_sym result_R0 bL).
+have -> //: Pr[CPA(Saber_PKE_Scheme, A).main() @ &m : res] = Pr[Game0(A).main() @ &m : res].
++ byequiv => //.
+  proc; inline *. 
+  swap {1} 7 -6.
+  call (_ : true); auto; call (_: true); auto.
+  progress; first do! congr; by rewrite pk_enc_dec_inv.
+  - by rewrite (eq_sym result_R0 bL).
 qed.
 
 (* Game0 <> Game1 ==> GMLWR *)
@@ -440,22 +440,22 @@ lemma Distinguish_Game0_Game1_To_GMLWR &m  (A <: Adversary) :
       = 
       `| Pr[GMLWR( B0(A) ).main(true) @ &m : res] - Pr[GMLWR( B0(A) ).main(false) @ &m : res] |. 
 proof.
-  have ->: Pr[Game0(A).main() @ &m : res] =  Pr[GMLWR( B0(A) ).main(false) @ &m : res].
-  + byequiv => //.
-    proc; inline *.
-    rcondf {2} 4.
-    - by move=> &m0; auto.
-    swap {2} 7 -6; wp.
-    by call (_ : true); auto; call (_: true); auto.
-  have ->: Pr[Game1(A).main() @ &m : res] =  Pr[GMLWR( B0(A) ).main(true) @ &m : res].
-  + byequiv => //.
-    proc; inline *.
-    rcondt {2} 4.
-    - by move=> &m0; auto.
-    swap {2} 7 -6; wp.
-    call (_ : true); auto; call (_: true); auto; rnd {2}; auto.
-    by progress; apply dsmallRq_vec_ll.
-  by apply distrC.
+have ->: Pr[Game0(A).main() @ &m : res] =  Pr[GMLWR( B0(A) ).main(false) @ &m : res].
++ byequiv => //.
+  proc; inline *.
+  rcondf {2} 4.
+  - by move=> &m0; auto.
+  swap {2} 7 -6; wp.
+  by call (_ : true); auto; call (_: true); auto.
+have ->: Pr[Game1(A).main() @ &m : res] =  Pr[GMLWR( B0(A) ).main(true) @ &m : res].
++ byequiv => //.
+  proc; inline *.
+  rcondt {2} 4.
+  - by move=> &m0; auto.
+  swap {2} 7 -6; wp.
+  call (_ : true); auto; call (_: true); auto; rnd {2}; auto.
+  by progress; apply dsmallRq_vec_ll.
+by apply distrC.
 qed.
 
 (* Game1 ==> Game2 *)
@@ -464,12 +464,184 @@ lemma Game1_To_Game2 &m (A <: Adversary) :
       =
       `| Pr[Game2( A2(A) ).main() @ &m : res] - 1%r / 2%r |.
 proof.
-  have -> //: Pr[Game1(A).main() @ &m : res] = Pr[Game2( A2(A) ).main() @ &m : res].
-  + byequiv => //.
-    proc; inline *.
-    wp; call (_ : true); auto; call (_ : true); auto.
-    by progress; do! congr; rewrite c_enc_dec_inv; 1: rewrite scaleRp2Rppq2R2t_comp.  
+have -> //: Pr[Game1(A).main() @ &m : res] = Pr[Game2( A2(A) ).main() @ &m : res].
++ byequiv => //.
+  proc; inline *.
+  wp; call (_ : true); auto; call (_ : true); auto.
+  by progress; do! congr; rewrite c_enc_dec_inv; 1: rewrite scaleRp2Rppq2R2t_comp.  
 qed.
+
+(*
+===========================================================================
+START TEST
+===========================================================================
+*)
+
+(* Game 2.5 *)
+module Game25(A : Adversary) = {
+   proc main() : bool = {
+      var u, u' : bool;
+      var m0, m1 : plaintext;
+
+      var sd : seed;
+      var _A : Rq_mat;
+      var s, s' : Rq_vec;
+      var bq : Rq_vec;
+      var b, b' : Rp_vec;
+      var v' : Rp;
+      var cmu : Rppq;
+
+      u <$ dbool;
+
+      sd <$ dseed;
+      _A <- gen sd;
+      (* Skip: s <$ dsmallRq_vec; *)
+      bq <$ dRq_vec;
+      b <- Rqv2Rpv bq;
+
+      (m0, m1) <@ A.choose(pk_encode (sd, b));
+
+      s' <$ dsmallRq_vec;
+      b' <- scaleRqv2Rpv ((trmx _A) *^ s' + h);
+      v' <- (dotp b (Rqv2Rpv s')) + (Rq2Rp h1);
+      cmu <- scaleRp2Rppq (v' + (shl_enc (m_decode (if u then m1 else m0)) (ep - 1)));
+      
+      u' <@ A.guess(c_encode (cmu, b'));
+
+      return (u = u');
+   }
+}.
+
+pragma Goals:printall.
+lemma Game25_To_Game3 &m (A <: Adversary) :
+      `| Pr[Game25(A).main() @ &m : res] - 1%r / 2%r |
+      =
+      `| Pr[Game3( A3(A) ).main() @ &m : res] - 1%r / 2%r |.
+proof.
+have -> //: Pr[Game25(A).main() @ &m : res] = Pr[Game3( A3(A) ).main() @ &m : res].
+byequiv => //.
+proc; inline *.
+auto; call(_ : true); auto; call(_ : true); auto.
+progress. 
++ by rewrite pk_enc_dec_inv. 
++ rewrite c_enc_dec_inv scaleRp2Rp_id //=. 
+  congr.
+  rewrite &(pw_eq) // cmu_red23.
+  do 2! congr.
+  by rewrite eq_sym (Rq2Rp_DM (dotp bqL s'L) h1) Rq2Rp_DotDl.
+qed.
+
+require import DMap.
+
+clone import DMapSampling with
+   type t1 <- Rq_vec,
+   type t2 <- Rp_vec.
+
+(* Game 2.4 *)
+module Game24(A : Adversary) = {
+   proc main() : bool = {
+      var u, u' : bool;
+      var m0, m1 : plaintext;
+
+      var sd : seed;
+      var _A : Rq_mat;
+      var s, s' : Rq_vec;
+      var b, b' : Rp_vec;
+      var v' : Rp;
+      var cmu : Rppq;
+
+      u <$ dbool;
+
+      sd <$ dseed;
+      _A <- gen sd;
+      (* Skip: s <$ dsmallRq_vec; *)
+      b <@ S.sample(dRq_vec, Rqv2Rpv);
+
+      (m0, m1) <@ A.choose(pk_encode (sd, b));
+
+      s' <$ dsmallRq_vec;
+      b' <- scaleRqv2Rpv ((trmx _A) *^ s' + h);
+      v' <- (dotp b (Rqv2Rpv s')) + (Rq2Rp h1);
+      cmu <- scaleRp2Rppq (v' + (shl_enc (m_decode (if u then m1 else m0)) (ep - 1)));
+      
+      u' <@ A.guess(c_encode (cmu, b'));
+
+      return (u = u');
+   }
+}.
+
+(* Game 2.6 *)
+module Game26(A : Adversary) = {
+   proc main() : bool = {
+      var u, u' : bool;
+      var m0, m1 : plaintext;
+
+      var sd : seed;
+      var _A : Rq_mat;
+      var s, s' : Rq_vec;
+      var bq : Rq_vec;
+      var b, b' : Rp_vec;
+      var v' : Rp;
+      var cmu : Rppq;
+
+      u <$ dbool;
+
+      sd <$ dseed;
+      _A <- gen sd;
+      (* Skip: s <$ dsmallRq_vec; *)
+      b <@ S.map(dRq_vec, Rqv2Rpv);
+
+      (m0, m1) <@ A.choose(pk_encode (sd, b));
+
+      s' <$ dsmallRq_vec;
+      b' <- scaleRqv2Rpv ((trmx _A) *^ s' + h);
+      v' <- (dotp b (Rqv2Rpv s')) + (Rq2Rp h1);
+      cmu <- scaleRp2Rppq (v' + (shl_enc (m_decode (if u then m1 else m0)) (ep - 1)));
+      
+      u' <@ A.guess(c_encode (cmu, b'));
+
+      return (u = u');
+   }
+}.
+
+
+lemma Game2_To_Game24 &m (A <: Adversary) :
+      `| Pr[Game2(A).main() @ &m : res] - 1%r / 2%r |
+      =
+      `| Pr[Game24(A).main() @ &m : res] - 1%r / 2%r |.
+proof.
+have -> //: Pr[Game2(A).main() @ &m : res] = Pr[Game24(A).main() @ &m : res].
+byequiv => //.
+proc; inline *.
+auto; call(_ : true); auto; call(_ : true); auto.
+progress.
+by rewrite dRqv2dRpv.
+rewrite dRqv2dRpv. apply /(is_fullP dRp_vec) /dRp_vec_fu.
+qed.
+
+lemma Game24_To_Game26 &m (A <: Adversary) :
+      `| Pr[Game24(A).main() @ &m : res] - 1%r / 2%r |
+      =
+      `| Pr[Game26(A).main() @ &m : res] - 1%r / 2%r |.
+proof.
+have -> //: Pr[Game24(A).main() @ &m : res] = Pr[Game26(A).main() @ &m : res].
+byequiv => //.
+proc. auto; call(_ : true); auto; call(_ : true). call (_ : ={d, f} ==> ={res}). rewrite sample.
+auto.
+qed.
+
+lemma Game26_To_Game25 &m (A <: Adversary) :
+      `| Pr[Game26(A).main() @ &m : res] - 1%r / 2%r |
+      =
+      `| Pr[Game25(A).main() @ &m : res] - 1%r / 2%r |.
+proof.
+have -> //: Pr[Game26(A).main() @ &m : res] = Pr[Game25(A).main() @ &m : res].
+byequiv => //.
+proc. inline *.
+auto; call(_ : true); auto; call(_ : true); auto.
+qed.
+
+(* ======================================================================= *)
 
 (* Game2 ==> Game3 *)
 lemma Game2_To_Game3 &m (A <: Adversary) :
@@ -477,22 +649,22 @@ lemma Game2_To_Game3 &m (A <: Adversary) :
       =
       `| Pr[Game3( A3(A) ).main() @ &m : res] - 1%r / 2%r |.
 proof.
-  have -> //: Pr[Game2(A).main() @ &m : res] = Pr[Game3( A3(A) ).main() @ &m : res].
-  + byequiv => //.
-    proc; inline *.
-    wp; call (_ : true); auto; call (_ : true); wp.
-    (* What functions to use here ... *)  
-    rnd (fun (pv : Rp_vec) => Rpv2Rqv pv)
-        (fun (pv : Rq_vec) => Rqv2Rpv pv).
-    auto; progress. 
-    - admit. 
-    - admit.
-    - by apply /(is_fullP dRq_vec) /dRq_vec_fu.
-    - by rewrite Rpv2Rqv_Rqv2Rpv_inv.
-    - by rewrite pk_enc_dec_inv /= Rpv2Rqv_Rqv2Rpv_inv.
-    - rewrite c_enc_dec_inv scaleRp2Rp_id //=; congr.
-      rewrite &(pw_eq) // cmu_red23 eq_sym; congr. 
-      by rewrite (Rq2Rp_DM (dotp (Rpv2Rqv bL) s'L) h1) Rq2Rp_DotDl Rpv2Rqv_Rqv2Rpv_inv.
+have -> //: Pr[Game2(A).main() @ &m : res] = Pr[Game3( A3(A) ).main() @ &m : res].
++ byequiv => //.
+  proc; inline *.
+  wp; call (_ : true); auto; call (_ : true); wp.
+  (* What functions to use here ... *)  
+  rnd (fun (pv : Rp_vec) => Rpv2Rqv pv)
+      (fun (pv : Rq_vec) => Rqv2Rpv pv).
+  auto; progress. 
+  - admit. 
+  - admit.
+  - by apply /(is_fullP dRq_vec) /dRq_vec_fu.
+  - by rewrite Rpv2Rqv_Rqv2Rpv_inv.
+  - by rewrite pk_enc_dec_inv /= Rpv2Rqv_Rqv2Rpv_inv.
+  - rewrite c_enc_dec_inv scaleRp2Rp_id //=; congr.
+    rewrite &(pw_eq) // cmu_red23 eq_sym; congr. 
+    by rewrite (Rq2Rp_DM (dotp (Rpv2Rqv bL) s'L) h1) Rq2Rp_DotDl Rpv2Rqv_Rqv2Rpv_inv.
 qed.
 
 (* Game3 <> Game4 ==> XMLWR *)
@@ -501,42 +673,42 @@ lemma Distinguish_Game3_Game4_To_XMLWR &m (A <: Adversary) :
       = 
       `| Pr[XMLWR( B1(A) ).main(true) @ &m : res] - Pr[XMLWR( B1(A) ).main(false) @ &m : res] |. 
 proof.
-  have ->: Pr[Game3(A).main() @ &m : res] =  Pr[XMLWR( B1(A) ).main(false) @ &m : res].
-  + byequiv => //.
-    proc; inline *.
-    rcondf {2} 4.
-    - by move => &m0; auto.
-    rcondf {2} 6.
-    - by move => &m0; auto.
-    swap {2} 11 -10; swap {1} 5 3; swap {2} 6 -2; wp.
-    by sim.
-  have ->: Pr[Game4(A).main() @ &m : res] =  Pr[XMLWR( B1(A) ).main(true) @ &m : res].
-  + byequiv => //.
-    proc; inline *.
-    rcondt {2} 4.
-    - by move => &m0; auto.
-    rcondt {2} 6.
-    - by move => &m0; auto.
-    swap {2} 11 -10; swap {1} 5 2; swap {2} 6 -1; wp.
-    sim; rnd {2}; auto.
-    by progress; apply dsmallRq_vec_ll.
-  by apply distrC.
+have ->: Pr[Game3(A).main() @ &m : res] =  Pr[XMLWR( B1(A) ).main(false) @ &m : res].
++ byequiv => //.
+  proc; inline *.
+  rcondf {2} 4.
+  - by move => &m0; auto.
+  rcondf {2} 6.
+  - by move => &m0; auto.
+  swap {2} 11 -10; swap {1} 5 3; swap {2} 6 -2; wp.
+  by sim.
+have ->: Pr[Game4(A).main() @ &m : res] =  Pr[XMLWR( B1(A) ).main(true) @ &m : res].
++ byequiv => //.
+  proc; inline *.
+  rcondt {2} 4.
+  - by move => &m0; auto.
+  rcondt {2} 6.
+  - by move => &m0; auto.
+  swap {2} 11 -10; swap {1} 5 2; swap {2} 6 -1; wp.
+  sim; rnd {2}; auto.
+  by progress; apply dsmallRq_vec_ll.
+by apply distrC.
 qed.
 
 (* Auxiliary_Game Analysis *)
 lemma Aux_Prob_Half &m  (A <: Adversary) :
       Pr[Auxiliary_Game(A).main() @ &m : res]  = 1%r / 2%r. 
 proof.
-  byphoare => //.
-  proc.
-  rnd. 
-  call (_: true); [apply (Adv_CPA_guess_ll A) | auto].
-  call(_ : true); [apply (Adv_CPA_choose_ll A) | auto].
-  by progress; [apply dseed_ll        |
-                apply dRq_vec_ll      |
-                apply dRp_vec_ll      |
-                apply Rp.dpolyXnD1_ll |
-                apply dbool1E].
+byphoare => //.
+proc.
+rnd. 
+call (_: true); [apply (Adv_CPA_guess_ll A) | auto].
+call(_ : true); [apply (Adv_CPA_choose_ll A) | auto].
+by progress; [apply dseed_ll        |
+              apply dRq_vec_ll      |
+              apply dRp_vec_ll      |
+              apply Rp.dpolyXnD1_ll |
+              apply dbool1E].
 qed.
 
 lemma Equivalence_Game4_Aux &m  (A <: Adversary) :
@@ -544,24 +716,24 @@ lemma Equivalence_Game4_Aux &m  (A <: Adversary) :
       =
       `| Pr[Auxiliary_Game(A).main() @ &m : res] - 1%r / 2%r |.
 proof.
-  have -> //: Pr[Game4(A).main() @ &m : res] = Pr[Auxiliary_Game(A).main() @ &m : res].
-  + byequiv => //. 
-    proc; inline *.
-    swap {2} 7 -6.
-    call (_ : true); wp.
-    rnd (fun (x : Rp) => x + (shl_enc (m_decode (if u{1} then m1{1} else m0{1})) (2 * ep - eq - 1)))  
-        (fun (x : Rp) => x - (shl_enc (m_decode (if u{1} then m1{1} else m0{1})) (2 * ep - eq - 1))).
-    auto; call(_ : true); auto.
-    progress.
-    - pose x := shl_enc (m_decode (if uL then result_R.`2 else result_R.`1)) (2 * ep - eq - 1).
-      by rewrite -addrA addNr addrC add0r. 
-    - by apply /rnd_funi /Rp.dpolyXnD1_funi.
-    - by apply /is_fullP /Rp.dpolyXnD1_fu.
-    - pose x := shl_enc (m_decode (if uL then result_R.`2 else result_R.`1)) (2 * ep - eq - 1).
-      have xx_0: forall (x : Rp), x + (- x) = Rp.zeroXnD1.
-      * by move => x0; rewrite -(addrN x0).
-      by rewrite -addrA (xx_0 x) addrC add0r.
-    - by rewrite scaleRp2Rp_id.  
+have -> //: Pr[Game4(A).main() @ &m : res] = Pr[Auxiliary_Game(A).main() @ &m : res].
++ byequiv => //. 
+  proc; inline *.
+  swap {2} 7 -6.
+  call (_ : true); wp.
+  rnd (fun (x : Rp) => x + (shl_enc (m_decode (if u{1} then m1{1} else m0{1})) (2 * ep - eq - 1)))  
+      (fun (x : Rp) => x - (shl_enc (m_decode (if u{1} then m1{1} else m0{1})) (2 * ep - eq - 1))).
+  auto; call(_ : true); auto.
+  progress.
+  - pose x := shl_enc (m_decode (if uL then result_R.`2 else result_R.`1)) (2 * ep - eq - 1).
+    by rewrite -addrA addNr addrC add0r. 
+  - by apply /rnd_funi /Rp.dpolyXnD1_funi.
+  - by apply /is_fullP /Rp.dpolyXnD1_fu.
+  - pose x := shl_enc (m_decode (if uL then result_R.`2 else result_R.`1)) (2 * ep - eq - 1).
+    have xx_0: forall (x : Rp), x + (- x) = Rp.zeroXnD1.
+    * by move => x0; rewrite -(addrN x0).
+    by rewrite -addrA (xx_0 x) addrC add0r.
+  - by rewrite scaleRp2Rp_id.  
 qed.
 
 (* Game4 Analysis *)
@@ -578,8 +750,8 @@ lemma Difference_Game1_Game4_To_XMLWR &m (A <: Adversary):
       =
       `| Pr[XMLWR( B1(A3(A2(A))) ).main(true) @ &m : res] - Pr[XMLWR( B1(A3(A2(A))) ).main(false) @ &m : res] |.
 proof. 
-  by rewrite (Game4_Prob_Half &m (A3(A2(A)))) (Game1_To_Game2 &m A) (Game2_To_Game3 &m (A2(A))) 
-            -(Game4_Prob_Half &m (A3(A2(A)))) (Distinguish_Game3_Game4_To_XMLWR &m (A3(A2(A)))).
+by rewrite (Game4_Prob_Half &m (A3(A2(A)))) (Game1_To_Game2 &m A) (Game2_To_Game3 &m (A2(A))) 
+          -(Game4_Prob_Half &m (A3(A2(A)))) (Distinguish_Game3_Game4_To_XMLWR &m (A3(A2(A)))).
 qed.
 
 (* Final Result (Security Theorem) *)
@@ -590,19 +762,19 @@ lemma Saber_INDCPA_Security_Theorem &m (A <: Adversary) :
       +
       `| Pr[XMLWR( B1(A3(A2(A))) ).main(true) @ &m : res] - Pr[XMLWR( B1(A3(A2(A))) ).main(false) @ &m : res] |. 
 proof.
-  rewrite (Equivalence_SaberINDCPA_Game0 &m A) -(Game4_Prob_Half &m (A3(A2(A)))).
-  have:
-       `| Pr[Game0(A).main() @ &m : res] - Pr[Game1(A).main() @ &m : res] |
-       +
-       `| Pr[Game1(A).main() @ &m : res] - Pr[Game4( A3(A2(A)) ).main() @ &m : res] |
-       <=
-       `| Pr[GMLWR(B0(A)).main(true) @ &m : res] - Pr[GMLWR(B0(A)).main(false) @ &m : res] | 
-       +
-       `| Pr[XMLWR(B1(A3(A2(A)))).main(true) @ &m : res] - Pr[XMLWR(B1(A3(A2(A)))).main(false) @ &m : res] |.
-  + by apply ler_add; [rewrite (Distinguish_Game0_Game1_To_GMLWR &m A) |
-                       rewrite -(Difference_Game1_Game4_To_XMLWR &m A) ].
-  move: (ler_dist_add (Pr[Game1(A).main() @ &m : res]) 
-                      (Pr[Game0(A).main() @ &m : res])
-                      (Pr[Game4( A3(A2(A)) ).main() @ &m : res])).
-  by apply ler_trans.  
+rewrite (Equivalence_SaberINDCPA_Game0 &m A) -(Game4_Prob_Half &m (A3(A2(A)))).
+have:
+     `| Pr[Game0(A).main() @ &m : res] - Pr[Game1(A).main() @ &m : res] |
+     +
+     `| Pr[Game1(A).main() @ &m : res] - Pr[Game4( A3(A2(A)) ).main() @ &m : res] |
+     <=
+     `| Pr[GMLWR(B0(A)).main(true) @ &m : res] - Pr[GMLWR(B0(A)).main(false) @ &m : res] | 
+     +
+     `| Pr[XMLWR(B1(A3(A2(A)))).main(true) @ &m : res] - Pr[XMLWR(B1(A3(A2(A)))).main(false) @ &m : res] |.
++ by apply ler_add; [rewrite (Distinguish_Game0_Game1_To_GMLWR &m A) |
+                     rewrite -(Difference_Game1_Game4_To_XMLWR &m A) ].
+move: (ler_dist_add (Pr[Game1(A).main() @ &m : res]) 
+                    (Pr[Game0(A).main() @ &m : res])
+                    (Pr[Game4( A3(A2(A)) ).main() @ &m : res])).
+by apply ler_trans.  
 qed.
